vtest-rocq/QEMU/ClintTimePass.v
@@ -21,7 +21,7 @@ Module ClintTimePass <: TEST_PASSES_AGREE ClintTime ClintTimeRun.
     cbn [ClintTimeRun.observed ClintTimeRun.results fmap list_fmap] in Ho.
     repeat (destruct Ho as [<-|Ho];
             [ apply (run_shows true lowest_head 8000);
-              vm_compute; repeat split |]).
+              vm_cast_no_check (eq_refl true) |]).
     destruct Ho.
   Qed.
 End ClintTimePass.
